Some specs for state initialization
In order to reason about the composition of partial states into a
complete state, in particular initial states, stronger specifications of
existing code are needed. Ideally, we want to ensure that initial states
"after linking" compose cleanly based on a disjoint set of components
owned by each program. Specifically, this observation should extend to
initial memories and program entry points.

Discussed with Guglielmo, who agrees while noting that the computational
component, mildly involved, made formalizing this reasoning cumbersome
at an early stage. Arthur may have had some ideas about alternative
designs back then, also according to Guglielmo, if I quote correctly.

It seems that these properties might be mildly annoying to prove, but
should hold. If it is the case that they do not hold, in all likelihood
the code, and not the specifications, should be amended to make this
property true, as otherwise state partitions along interface lines would
become difficult and unintuitive.

Intermediate/Machine.v
@@ -532,6 +532,36 @@ Proof.
   apply alloc_static_buffers_after_linking; auto.
 Qed.
 
+Definition prepare_procedures_memory (p: program) (mem: Memory.t) : Memory.t :=
+  let '(mem, _, _) := prepare_procedures p mem in
+  mem.
+
+Theorem prepare_procedures_memory_after_linking:
+  forall p c,
+    well_formed_program p ->
+    well_formed_program c ->
+    linkable (prog_interface p) (prog_interface c) ->
+    prepare_procedures_memory (program_link p c)
+                              (prepare_initial_memory (program_link p c)) =
+    unionm (prepare_procedures_memory p (prepare_initial_memory p))
+           (prepare_procedures_memory c (prepare_initial_memory c)).
+Admitted.
+
+Definition prepare_procedures_entrypoints (p: program) (mem: Memory.t) : EntryPoint.t :=
+  let '(_, _, entrypoints) := prepare_procedures p mem in
+  entrypoints.
+
+Theorem prepare_procedures_entrypoints_after_linking:
+  forall p c,
+    well_formed_program p ->
+    well_formed_program c ->
+    linkable (prog_interface p) (prog_interface c) ->
+    prepare_procedures_entrypoints (program_link p c)
+                                   (prepare_initial_memory (program_link p c)) =
+    unionm (prepare_procedures_entrypoints p (prepare_initial_memory p))
+           (prepare_procedures_entrypoints c (prepare_initial_memory c)).
+Admitted.
+
 Lemma link_sym:
   forall p c,
     well_formed_program p ->
